src/ChipTactics.v
@@ -1,0 +1,65 @@
+Require Import Integers.
+Require Import Coqlib.
+Require Import Maps.
+
+Import Int.
+Require Import Hardware.
+
+Ltac dec_eq_try :=
+  repeat (rewrite dec_eq_false;
+    [ idtac | solve [ let F := fresh in (intro F; inversion F)] ] +
+  rewrite dec_eq_true + fail).
+
+Ltac simpl_code :=
+  repeat autounfold with chipmem; simpl;
+  repeat match goal with
+  | |- context[add (repr ?x) (repr ?y)] =>
+    let GR := fresh in assert (GR: add (repr x) (repr y) = repr (x + y)) by
+      (rewrite add_unsigned; rewrite unsigned_repr_eq; rewrite <- Z_mod_modulus_eq;
+      apply f_equal; auto); rewrite GR; clear GR; simpl
+  | |- context[?x # ?y <- ?z] =>
+    change (x # y <- z) with (RegMap.set y z x); try unfold RegMap.set
+  end; repeat autounfold with chipmem; simpl.
+
+Ltac deal_with_eq_dec :=
+  repeat (let F := fresh in
+   (case (eq_dec _ _); intro F; try inversion F));
+  repeat match goal with
+  | |- context[Reg_eq ?x ?x] =>
+    rewrite dec_eq_true
+  | H: context[Reg_eq ?x ?x] |- _ =>
+    rewrite dec_eq_true in H; try rewrite H
+  end; repeat (case (Reg_eq _ _); intros).
+
+Ltac inverse_eq :=
+  match goal with
+  | H: ?x = ?y |- _ => try inversion H
+  end.
+
+Ltac deal_with_eq :=
+  repeat match goal with
+  | |- context [eq ?x ?x] =>
+    rewrite Z_eq_eq
+  | H: context[eq ?x ?x] |- _ =>
+    rewrite Z_eq_eq in H
+  end; autounfold with Z_unfold;
+  try (case (Z.eq_dec _ _); intros; [intuition | inverse_eq]); simpl in *.
+
+Ltac Fine_eq :=
+  match goal with
+  | |- context[Fine ?M' ?IM' ?RF' ?St' = Fine _ _ _ _ /\ _] =>
+    exists M'; exists IM'; exists RF'; exists St'
+  end.
+
+Lemma rsb_is_reverse_sub: forall M IM RF St v v',
+  (IM (RF#PC)) = (Isub v v') ->
+  let EIMsub := ExecuteStep M IM RF St in
+  let EIMrsb := ExecuteStep M (InstructionMap.set (RF#PC) (Irsb v' v) IM) RF St in
+  OutputM EIMsub = OutputM EIMrsb /\
+  OutputRF EIMsub = OutputRF EIMrsb /\
+  OutputStack EIMsub = OutputStack EIMrsb.
+Proof.
+  intros. subst EIMsub. subst EIMrsb.
+  simpl_code. rewrite H. simpl.
+  dec_eq_try. auto.
+Qed.
